src/spec/TLS13.Wire.Spec.fst
@@ -502,6 +502,17 @@ let parse_ignored_post_handshake (input:B.bytes) : GTot (option B.bytes) =
     then Some (Seq.slice input 4 (body_len + 4))
     else None
 
+let parse_key_update (input:B.bytes) : GTot (option M.key_update_request) =
+  if B.length input == 5 &&
+     nat_of_byte (Seq.index input 0) == 24 &&
+     read_u24 input 1 == 1
+  then
+    let request = nat_of_byte (Seq.index input 4) in
+    if request == 0 then Some M.UpdateNotRequested
+    else if request == 1 then Some M.UpdateRequested
+    else None
+  else None
+
 let parse_handshake (input:B.bytes) : GTot (option (M.handshake_msg & nat)) =
   if B.length input < 4 then None
   else
@@ -876,9 +887,12 @@ let parse_tls_message (content_type:T.content_type) (fragment:B.bytes) : GTot (o
      | Some (msg, consumed) ->
        if consumed == B.length fragment then Some (M.TlsHandshake msg) else None
      | None ->
-       match parse_ignored_post_handshake fragment with
-       | Some body -> Some (M.TlsIgnoredPostHandshake body)
-       | None -> None)
+       match parse_key_update fragment with
+       | Some req -> Some (M.TlsKeyUpdate req)
+       | None ->
+         match parse_ignored_post_handshake fragment with
+         | Some body -> Some (M.TlsIgnoredPostHandshake body)
+         | None -> None)
   | T.ApplicationData -> Some (M.TlsApplicationData fragment)
   | T.Alert ->
     if B.length fragment == 2
@@ -899,6 +913,12 @@ let serialize_tls_message (msg:M.tls_message) : GTot (T.content_type & B.bytes) 
   | M.TlsAlert alert -> (T.Alert, B.of_list [byte 2; byte (alert_description_to_byte alert)])
   | M.TlsChangeCipherSpec -> (T.ChangeCipherSpec, B.singleton (byte 1))
   | M.TlsIgnoredPostHandshake body -> (T.Handshake, append3 (u8 4) (u24 (B.length body)) body)
+  | M.TlsKeyUpdate req ->
+    let request_byte =
+      match req with
+      | M.UpdateNotRequested -> 0
+      | M.UpdateRequested -> 1 in
+    (T.Handshake, append3 (u8 24) (u24 1) (u8 request_byte))
 
 let parse_tls_record (input:B.bytes) : GTot (option (M.tls_record & nat)) =
   match parse_record input with
